Fixing coherence for external events.

Coherence.v
@@ -1,7 +1,7 @@
 Require Import CSet Le.
 
 Require Import Plus Util AllInRel Map.
-Require Import Val Var Env EnvTy IL Annotation Liveness ParamsMatch Restrict Sim MoreExp.
+Require Import Val Var Env EnvTy IL Annotation Liveness Restrict Bisim MoreExp.
 
 Set Implicit Arguments.
 
@@ -32,10 +32,10 @@ Qed.
 
 Inductive ssa : stmt -> ann (set var * set var) -> Prop :=
   | ssaExp x e s D D' an
-    : x ∉ D 
+    : x ∉ D
       -> Exp.freeVars e ⊆ D
       -> ssa s an
-      -> pe (getAnn an) (D ∪ {{x}}, D') 
+      -> pe (getAnn an) (D ∪ {{x}}, D')
       -> ssa (stmtExp x e s) (ann1 (D, D') an)
   | ssaIf  D D' Ds Dt e s t ans ant
     : Exp.freeVars e ⊆ D
@@ -51,14 +51,20 @@ Inductive ssa : stmt -> ann (set var * set var) -> Prop :=
       -> D [=] D'
       -> ssa (stmtReturn e) (ann0 (D, D'))
   | ssaGoto D D' f Y
-    : list_union (List.map Exp.freeVars Y) ⊆ D 
+    : list_union (List.map Exp.freeVars Y) ⊆ D
       -> D [=] D'
       -> ssa (stmtGoto f Y) (ann0 (D, D'))
+  | ssaExtern x f Y s D D' an
+    : x ∉ D
+      -> list_union (List.map Exp.freeVars Y) ⊆ D
+      -> ssa s an
+      -> pe (getAnn an) (D ∪ {{x}}, D')
+      -> ssa (stmtExtern x f Y s) (ann1 (D, D') an)
   | ssaLet D D' s t Ds Dt Z ans ant
     : of_list Z ∩ D [=] ∅
       -> Ds ∩ Dt [=] D
       -> Ds ∪ Dt [=] D'
-      -> ssa s ans 
+      -> ssa s ans
       -> pe (getAnn ans) (of_list Z ∪ D, Ds)
       -> ssa t ant
       -> pe (getAnn ant) (D, Dt)
@@ -84,20 +90,24 @@ Lemma ssa_ext s an an'
   : ann_R pe an an'
   -> ssa s an
   -> ssa s an'.
-Proof. 
+Proof.
   intros. general induction H0; simpl; invt (ann_R pe); invt pe; eauto using ssa.
   - econstructor. rewrite <- H7; eauto. rewrite <- H7; eauto.
-    eapply IHssa; eauto. rewrite <- H7. rewrite (ann_R_get H8) in H2. 
+    eapply IHssa; eauto. rewrite <- H7. rewrite (ann_R_get H8) in H2.
     rewrite <- H10. eauto.
-  
-  - econstructor. rewrite <- H7; eauto. rewrite <- H7; eauto. rewrite H1; eauto. 
+
+  - econstructor. rewrite <- H7; eauto. rewrite <- H7; eauto. rewrite H1; eauto.
     eapply IHssa1; eauto; reflexivity.
     eapply IHssa2; eauto; reflexivity.
     rewrite <- (ann_R_get H10). rewrite <- H7. eauto.
     rewrite <- (ann_R_get H11). rewrite <- H7. eauto.
-  
+
   - econstructor. rewrite <- H5; eauto. rewrite <- H5, <- H7; eauto.
   - econstructor. rewrite <- H5; eauto. rewrite <- H5, <- H7; eauto.
+
+  - econstructor. rewrite <- H7; eauto. rewrite <- H7; eauto.
+    eapply IHssa; eauto. rewrite <- H7, <- H10.
+    rewrite <- (ann_R_get H8). eauto.
 
   - econstructor. rewrite <- H7; eauto.
     rewrite <- H7; eauto.
@@ -113,17 +123,18 @@ Proof.
   eapply ssa_ext; eauto.
   eapply ssa_ext; try symmetry; eauto.
 Qed.
- 
+
 Lemma ssa_incl s an
   : ssa s an -> fst (getAnn an) ⊆ snd (getAnn an).
-Proof. 
+Proof.
   intros. general induction H; eauto using ssa; simpl; cset_tac; eauto.
-  - destruct (getAnn an); simpl in *. inv H2. rewrite <- H9. 
-    eapply IHssa. rewrite H7. cset_tac; eauto.
-  - destruct (getAnn ans); destruct (getAnn ant); simpl in *.
-    inv H4; inv H5. eapply H1. eapply H0 in H6. intuition.
+  - rewrite H2 in IHssa; simpl in *. rewrite <- IHssa. cset_tac; intuition.
+  - rewrite H4 in IHssa1. rewrite H5 in IHssa2. simpl in *.
+    eapply H1; eauto.
   - eapply H0; eauto.
   - eapply H0; eauto.
+  - rewrite H2 in IHssa; simpl in *.
+    eapply IHssa. cset_tac; intuition.
   - eapply H1. eapply H0 in H6. left; eapply H6.
 Qed.
 
@@ -131,11 +142,12 @@ Lemma ssa_freeVars s an
   : ssa s an -> freeVars s ⊆ fst (getAnn an).
 Proof.
   intros. general induction H; simpl; eauto.
-  - rewrite H0, IHssa. inv H2; simpl. rewrite H6. 
+  - rewrite H0, IHssa, H2. simpl.
     clear_all; cset_tac; intuition.
-  - rewrite H, IHssa1, IHssa2. inv H4; inv H5; simpl.
-    rewrite H9, H12. cset_tac; intuition.
-  - rewrite IHssa1, IHssa2. inv H3; inv H5; simpl. 
+  - rewrite H, IHssa1, IHssa2. rewrite H4, H5; simpl.
+    cset_tac; intuition.
+  - rewrite H0, IHssa, H2; simpl. cset_tac; intuition.
+  - rewrite IHssa1, IHssa2. inv H3; inv H5; simpl.
     rewrite H9, H12. cset_tac; intuition.
 Qed.
 
@@ -159,8 +171,8 @@ Proof.
     rewrite H0, H2. reflexivity.
 Qed.
 
-Definition pminus (D'':set var) s := 
-  match s with 
+Definition pminus (D'':set var) s :=
+  match s with
     | pair s s' => (s \ D'', s' \ D'')
   end.
 
@@ -173,7 +185,7 @@ Proof.
     + eapply Exp.notOccur_freeVars in H9; eauto. rewrite meet_comm in H9.
       rewrite <- H0. rewrite minus_inane_set; eauto. reflexivity.
     + eapply IHssa; eauto.
-    + rewrite getAnn_mapAnn. inv H2; simpl. 
+    + rewrite getAnn_mapAnn. inv H2; simpl.
       rewrite H10, H11. econstructor. cset_tac; intuition.
       eapply H7. rewrite <- H6; eauto.
       reflexivity.
@@ -186,48 +198,53 @@ Proof.
     reflexivity.
     rewrite getAnn_mapAnn. inv H3; simpl. rewrite H11, H12.
     reflexivity.
-  - econstructor. 
-    eapply Exp.notOccur_freeVars in H3. 
+  - econstructor.
+    eapply Exp.notOccur_freeVars in H3.
     rewrite meet_comm in H3.
     rewrite <- H. rewrite minus_inane_set; eauto. reflexivity.
     rewrite H0. reflexivity.
   - econstructor. unfold list_union.
     hnf; intros. eapply list_union_get in H2.
     destruct H2 as [[? []]|]; dcr. edestruct map_get_4; eauto; dcr; subst.
-    exploit H3; eauto. 
+    exploit H3; eauto.
     eapply Exp.notOccur_freeVars in H3; eauto. rewrite meet_comm in H3.
     cset_tac; intuition.
     rewrite <- H. eapply incl_list_union; eauto. reflexivity.
     eauto. cset_tac; intuition. rewrite H0; reflexivity.
-  - econstructor; eauto. 
+  - econstructor; eauto.
     revert H H8; clear_all; cset_tac; intuition; eauto.
     rewrite <- H0. rewrite minus_dist_intersection. reflexivity.
     rewrite <- H1. rewrite minus_dist_union. reflexivity.
     rewrite getAnn_mapAnn; simpl. inv H2; simpl.
-    rewrite H11, H12. constructor; try reflexivity. 
+    rewrite H11, H12. constructor; try reflexivity.
     revert H8; clear_all; cset_tac; intuition; eauto.
     rewrite getAnn_mapAnn; simpl. inv H3; simpl.
-    rewrite H11, H12. reflexivity. 
+    rewrite H11, H12. reflexivity.
 Qed.
 
 (* shadowing free *)
 Inductive shadowing_free : set var -> stmt -> Prop :=
   | shadowing_freeExp x e s D
-    : x ∉ D 
+    : x ∉ D
       -> Exp.freeVars e ⊆ D
       -> shadowing_free (D ∪ {{x}}) s
       -> shadowing_free D (stmtExp x e s)
   | shadowing_freeIf D e s t
     : Exp.freeVars e ⊆ D
-    -> shadowing_free D s 
+    -> shadowing_free D s
     -> shadowing_free D t
     -> shadowing_free D (stmtIf e s t)
   | shadowing_freeRet D e
     : Exp.freeVars e ⊆ D
     -> shadowing_free D (stmtReturn e)
   | shadowing_freeGoto D f Y
-    : list_union (List.map Exp.freeVars Y) ⊆ D 
+    : list_union (List.map Exp.freeVars Y) ⊆ D
     -> shadowing_free D (stmtGoto f Y)
+  | shadowing_freeExtern x f Y s D
+    : x ∉ D
+      -> list_union (List.map Exp.freeVars Y) ⊆ D
+      -> shadowing_free (D ∪ {{x}}) s
+      -> shadowing_free D (stmtExtern x f Y s)
   | shadowing_freeLet D s t Z
     : of_list Z ∩ D [=] ∅
     -> shadowing_free (of_list Z ∪ D) s
@@ -238,10 +255,11 @@ Lemma shadowing_free_ext s D D'
   : D' [=] D
   -> shadowing_free D s
   -> shadowing_free D' s.
-Proof. 
+Proof.
   intros EQ SF. general induction SF; simpl; econstructor; try rewrite EQ; eauto.
-  - eapply IHSF; eauto. 
+  - eapply IHSF; eauto.
     rewrite EQ; reflexivity.
+  - eapply IHSF; eauto. rewrite EQ; reflexivity.
   - eapply IHSF1; eauto. rewrite EQ. reflexivity.
 Qed.
 
@@ -255,11 +273,12 @@ Qed.
 Lemma ssa_shadowing_free s an
   : ssa s an -> shadowing_free (fst (getAnn an)) s.
 Proof.
-  intros. general induction H; simpl; try invt pe; eauto using shadowing_free.
+  intros. general induction H; simpl; eauto using shadowing_free.
   - econstructor; eauto. rewrite H2 in IHssa. eauto.
-  - rewrite H4 in IHssa1. rewrite H5 in IHssa2. 
+  - rewrite H4 in IHssa1. rewrite H5 in IHssa2.
     econstructor; eauto.
-  - rewrite H3 in IHssa1. rewrite H5 in IHssa2. 
+  - econstructor; eauto. rewrite H2 in IHssa; eauto.
+  - rewrite H3 in IHssa1. rewrite H5 in IHssa2.
     econstructor; eauto.
 Qed.
 
@@ -278,6 +297,9 @@ Inductive srd : list (option (set var)) -> stmt -> ann (set var) -> Prop :=
     : get DL (counted f) (Some G')
     -> G' ⊆ lv
     -> srd DL (stmtGoto f Y) (ann0 lv)
+ | srdExtern DL x f Y s lv al
+    : srd (restrict DL (lv\{{x}})) s al
+    -> srd DL (stmtExtern x f Y s) (ann1 lv al)
   | srdLet DL s t Z lv als alt
     : srd (restrict (Some (getAnn als \ of_list Z)::DL) (getAnn als \ of_list Z))
           s als
@@ -287,28 +309,28 @@ Inductive srd : list (option (set var)) -> stmt -> ann (set var) -> Prop :=
 Definition peq := prod_eq (@feq var var eq) (@Equal var _ _).
 
 (*
-Instance srd_morphism 
+Instance srd_morphism
   : Proper (list_eq (option_eq Equal) ==> Equal ==> eq ==> impl) srd.
 Proof.
   unfold Proper, peq, respectful, impl; intros; decompose records; simpl in *; subst.
   general induction H2; simpl in *; eauto using srd.
-  + econstructor; eauto. 
+  + econstructor; eauto.
     - rewrite <- H1; eauto.
     - eapply IHsrd. rewrite H0. rewrite <- H1. reflexivity.
       rewrite H1. reflexivity.
-  
+
   + econstructor; eauto. rewrite <- H1; eauto.
   + econstructor; eauto. rewrite <- H1; eauto.
 
-  + edestruct (list_eq_get H2 H0); decompose records; 
+  + edestruct (list_eq_get H2 H0); decompose records;
     destruct x; simpl in * |- *; eauto; inv H6.
     econstructor; eauto. rewrite <- H3; eauto.
     rewrite <- H3, <- H8; eauto.
-    
+
   + econstructor; eauto. rewrite <- H1; eauto.
     eapply IHsrd1; eauto; try reflexivity.
     econstructor; eauto. reflexivity.
-    rewrite H0. reflexivity. 
+    rewrite H0. reflexivity.
     eapply IHsrd2; eauto. constructor; eauto; reflexivity.
 Qed.
 *)
@@ -342,77 +364,77 @@ Proof.
     case_eq (is_empty s); intros.
     right; intro A; inv A. assert (G' ∈ s). unfold s.
     rewrite filter_iff. split. eapply powerset_spec; eauto.
-    eapply andb_true_iff; split. 
-    destruct (IHs2 ((Some G') :: DL) G); simpl; eauto. 
+    eapply andb_true_iff; split.
+    destruct (IHs2 ((Some G') :: DL) G); simpl; eauto.
     destruct (IHs1 (restrict ((Some G') :: DL) G') (G' ∪ of_list Z)); simpl; eauto.
 
     Opaque restrict.
-    hnf; intros. simpl. 
-    clear H. clear s. 
-    destruct (IHs2 ((Some x) :: DL) G), 
+    hnf; intros. simpl.
+    clear H. clear s.
+    destruct (IHs2 ((Some x) :: DL) G),
              (IHs1 (restrict ((Some x) :: DL) x) (x ∪ of_list Z)),
              (IHs2 ((Some y) :: DL) G),
              (IHs1 (restrict ((Some y) :: DL) y) (y ∪ of_list Z));
-      simpl; eauto. 
+      simpl; eauto.
     eapply srd_morphism in s0; eauto.
-    exfalso; eauto. 
-    repeat (rewrite restrict_incl; try reflexivity). 
+    exfalso; eauto.
+    repeat (rewrite restrict_incl; try reflexivity).
     econstructor; eauto. econstructor; eauto. rewrite H0. reflexivity.
     rewrite <- H0. reflexivity.
     eapply srd_morphism in s; eauto.
-    exfalso; eauto. econstructor; eauto. econstructor; eauto. 
-    reflexivity. reflexivity. 
+    exfalso; eauto. econstructor; eauto. econstructor; eauto.
+    reflexivity. reflexivity.
     eapply srd_morphism in s; eauto.
-    exfalso; eauto. econstructor; eauto. econstructor; eauto. 
-    reflexivity. reflexivity. 
+    exfalso; eauto. econstructor; eauto. econstructor; eauto.
+    reflexivity. reflexivity.
     eapply srd_morphism in s3; eauto.
-    repeat (rewrite restrict_incl; try reflexivity). 
+    repeat (rewrite restrict_incl; try reflexivity).
     econstructor; eauto. econstructor; eauto. symmetry; eauto.
-    rewrite H0; reflexivity. rewrite H0; reflexivity. 
+    rewrite H0; reflexivity. rewrite H0; reflexivity.
     eapply srd_morphism in s0; eauto.
     econstructor; eauto. econstructor; eauto. symmetry; eauto.
-    reflexivity. reflexivity. 
+    reflexivity. reflexivity.
     eapply srd_morphism in s; eauto.
     econstructor; eauto. econstructor; eauto. symmetry; eauto.
     reflexivity. reflexivity.
-    
+
     eapply is_empty_iff in H. eapply empty_is_empty_1 in H.  cset_tac; eauto.
     case_eq (choose s). intros G' ?.
     eapply choose_1 in H0. unfold s in H0.
     eapply filter_iff in H0. rewrite andb_true_iff in H0. dcr.
     Opaque restrict.
     destruct (IHs2 ((Some G') :: DL) G); simpl in *; eauto; try congruence.
-    destruct (IHs1 (restrict ((Some G') :: DL) G') (G' ∪ of_list Z)); 
+    destruct (IHs1 (restrict ((Some G') :: DL) G') (G' ∪ of_list Z));
       simpl in *; eauto; try congruence.
     eapply powerset_spec in H1.
     left. econstructor; eauto.
 
-    hnf; intros. simpl. 
-    clear H. clear s. 
-    destruct (IHs2 ((Some x) :: DL) G), 
+    hnf; intros. simpl.
+    clear H. clear s.
+    destruct (IHs2 ((Some x) :: DL) G),
              (IHs1 (restrict ((Some x) :: DL) x) (x ∪ of_list Z)),
              (IHs2 ((Some y) :: DL) G),
              (IHs1 (restrict ((Some y) :: DL) y) (y ∪ of_list Z));
       simpl; eauto.
     eapply srd_morphism in s0; eauto.
-    exfalso; eauto. 
-    repeat (rewrite restrict_incl; try reflexivity). 
-    econstructor; eauto. econstructor; eauto. 
+    exfalso; eauto.
+    repeat (rewrite restrict_incl; try reflexivity).
+    econstructor; eauto. econstructor; eauto.
     rewrite <- H1. reflexivity. rewrite H1; reflexivity.
     eapply srd_morphism in s; eauto.
-    exfalso; eauto. econstructor; eauto. econstructor; eauto. 
-    reflexivity. reflexivity. 
+    exfalso; eauto. econstructor; eauto. econstructor; eauto.
+    reflexivity. reflexivity.
     eapply srd_morphism in s; eauto.
-    exfalso; eauto. econstructor; eauto. econstructor; eauto. 
-    reflexivity. reflexivity. 
+    exfalso; eauto. econstructor; eauto. econstructor; eauto.
+    reflexivity. reflexivity.
     eapply srd_morphism in s3; eauto.
-    repeat (rewrite restrict_incl; try reflexivity). 
-    econstructor; eauto. econstructor; eauto; try reflexivity. 
+    repeat (rewrite restrict_incl; try reflexivity).
+    econstructor; eauto. econstructor; eauto; try reflexivity.
     rewrite H1; reflexivity. rewrite H1; reflexivity.
     rewrite H1; reflexivity.
     eapply srd_morphism in s0; eauto.
     econstructor; eauto. econstructor; eauto. symmetry; eauto.
-    reflexivity. reflexivity. 
+    reflexivity. reflexivity.
     eapply srd_morphism in s; eauto.
     econstructor; eauto. econstructor; eauto. symmetry; eauto.
     reflexivity. reflexivity.
@@ -422,7 +444,7 @@ Qed.
 *)
 Transparent restrict.
 
-
+(*
 Fixpoint freeVar_live (s:stmt) : ann (set var) :=
   match s with
     | stmtExp x e s0 => ann1 (freeVars s) (freeVar_live s0)
@@ -438,13 +460,13 @@ Proof.
   destruct s; eauto.
 Qed.
 
-(*
+
 Lemma free_live_sound s Lv DL D G
   : (forall n blv Z, get Lv n (blv, Z) -> of_list Z ⊆ blv)
   -> srd DL (D, G) s
-  -> live_sound Lv s (freeVar_live s). 
+  -> live_sound Lv s (freeVar_live s).
 Proof.
-  intros. general induction H0; simpl in * |- *. 
+  intros. general induction H0; simpl in * |- *.
   econstructor. eapply IHsrd; eauto. eapply union_subset_2.
   rewrite getAnn_freeVar_live. eapply union_subset_1.
   econstructor; eauto. eapply union_subset_2; cset_tac; eauto.
@@ -457,16 +479,18 @@ Abort.
 *)
 
 Lemma srd_monotone (DL DL' : list (option (set var))) s a
- : srd DL s a 
+ : srd DL s a
    -> list_eq (fstNoneOrR Equal) DL DL'
    -> srd DL' s a.
 Proof.
   intros. general induction H; eauto using srd.
-  + econstructor. 
-    eapply IHsrd; eauto. eapply restrict_subset; eauto. cset_tac; intuition.
+  + econstructor.
+    eapply IHsrd; eauto. eapply restrict_subset; eauto. reflexivity.
   + destruct (list_eq_get H1 H); eauto; dcr. inv H4.
     econstructor; eauto. rewrite <- H5; eauto.
-  + econstructor; eauto. 
+  + econstructor. eapply IHsrd; eauto.
+    eapply restrict_subset; eauto. reflexivity.
+  + econstructor; eauto.
     eapply IHsrd1. repeat rewrite restrict_incl; try reflexivity.
     constructor; eauto. reflexivity.
     eapply restrict_subset; eauto. reflexivity.
@@ -474,16 +498,17 @@ Proof.
 Qed.
 
 Lemma srd_monotone2 (DL DL' : list (option (set var))) s a
- : srd DL s a 
+ : srd DL s a
    -> list_eq (fstNoneOrR (flip Subset)) DL DL'
    -> srd DL' s a.
 Proof.
   intros. general induction H; eauto using srd.
-  + econstructor. 
+  + econstructor.
     eapply IHsrd; eauto. eapply restrict_subset2; eauto. reflexivity.
   + destruct (list_eq_get H1 H); eauto; dcr. inv H4.
     econstructor; eauto. rewrite <- H5; eauto.
-  + econstructor; eauto. 
+  + econstructor. eapply IHsrd, restrict_subset2; eauto. reflexivity.
+  + econstructor; eauto.
     eapply IHsrd1. repeat rewrite restrict_incl; try reflexivity.
     constructor; eauto. reflexivity.
     eapply restrict_subset2; eauto. reflexivity.
@@ -500,7 +525,7 @@ Lemma shadowing_free_srd G s DL
 Proof.
   intros. general induction H; inv A; eauto using srd.
 
-  + econstructor; eauto. eapply IHshadowing_free; eauto. 
+  + econstructor; eauto. eapply IHshadowing_free; eauto.
     unfold restrict. eapply labl_other; try eassumption.
     rewrite map_length; eauto.
     eapply bounded_restrict. cset_tac; intuition.
@@ -508,7 +533,7 @@ Proof.
     intro. eapply H; rewrite H4 in H3; eauto. rewrite <- H3 in H2.
     erewrite bounded_restrict_eq in H2; try eapply B; try reflexivity.
     eapply C; eauto.
- 
+
   + destruct y. econstructor; eauto. eapply bounded_get; eauto. eapply C in H2. congruence.
   + assert (D [=] D \ of_list Z) by (cset_tac; intuition eauto).
     econstructor; eauto.
@@ -518,7 +543,7 @@ Proof.
       rewrite <- H2 at 2.
       eapply IHshadowing_free1. eapply labl_other; try eassumption; simpl; f_equal.
       simpl. split. cset_tac; intuition. eapply bounded_morphism_subset; eauto; cset_tac; intuition.
-      intros. inv H3. congruence. eapply C; eauto. reflexivity. 
+      intros. inv H3. congruence. eapply C; eauto. reflexivity.
       simpl; split; try reflexivity. rewrite <- H2; eauto.
     - eapply IHshadowing_free2. eapply labl_other; try eassumption; simpl; f_equal.
       simpl; split; eauto using minus_incl.
@@ -527,7 +552,7 @@ Qed.
 *)
 
 Definition invariant (s:stmt) :=
-  forall (E:onv var), sim (nil:list F.block,E,s) (nil:list I.block,E,s).
+  forall (E:onv var), bisim (nil:list F.block,E,s) (nil:list I.block,E,s).
 
 Definition rd_agree (DL:list (option (set var)))
            L (E:onv val)
@@ -539,7 +564,7 @@ Lemma rd_agree_update DL L E G x v
  (RA:rd_agree DL L E)
   : rd_agree (restrict DL (G \ {{x}})) L (E [x <- v]).
 Proof.
-  intros. hnf; intros. 
+  intros. hnf; intros.
   unfold restrict in H0. eapply map_get_4 in H0; dcr.
   unfold restr in H2. destruct x0; isabsurd. destruct if in H2; isabsurd.
   inv H2. eapply agree_on_update_dead. rewrite s0. cset_tac; intuition.
@@ -554,13 +579,13 @@ Lemma rd_agree_update_list DL L E E' (G G':set var) Z n vl
 : rd_agree (restrict (drop n DL) G') (drop n L) (E'[Z <-- vl]).
 Proof.
   hnf; intros.
-  assert (G'0 ⊆ G'). { 
+  assert (G'0 ⊆ G'). {
     eapply bounded_get; eauto. eapply bounded_restrict; reflexivity.
-  } 
+  }
   assert (G'0 [=] G'0 \ of_list Z) by (split; cset_tac; intuition eauto).
-  rewrite H2. eapply update_with_list_agree_minus; eauto. 
+  rewrite H2. eapply update_with_list_agree_minus; eauto.
 
-  unfold restrict in H0. rewrite drop_map in H0. 
+  unfold restrict in H0. rewrite drop_map in H0.
   eapply get_drop in H. eapply get_drop in H0.
   eapply map_get_4 in H0; dcr.
   hnf in RA.
@@ -570,11 +595,11 @@ Proof.
 Qed.
 
 
-Inductive approx' 
+Inductive approx'
   : list (option (set var)) -> F.block -> Prop :=
   approxI' DL o Z E s DL'
   :  (forall G, o = Some G -> of_list Z ∩ G [=] ∅ /\
-           exists a, getAnn a [=] (G ∪ of_list Z) 
+           exists a, getAnn a [=] (G ∪ of_list Z)
                 /\ srd (restrict (Some G::DL) G) s a
                 /\ live_sound DL' s a)
      -> approx' (o::DL) (F.blockI E Z s).
@@ -589,22 +614,22 @@ Proof.
   inv pf. econstructor.
   intros. inv H1.
   eapply restr_iff in H0; dcr; subst.
-  specialize (H4 _ H1); dcr. 
-  rewrite restrict_incl, restrict_idem, <- restrict_incl; eauto; try reflexivity.   
-  inv pf. econstructor. isabsurd. eapply IHAIR2; eauto. 
+  specialize (H4 _ H1); dcr.
+  rewrite restrict_incl, restrict_idem, <- restrict_incl; eauto; try reflexivity.
+  inv pf. econstructor. isabsurd. eapply IHAIR2; eauto.
   Grab Existential Variables. eassumption.
 Qed.
 
 Unset Printing Records.
 
-Lemma srd_preservation (E E':onv val) L L' s s' DL (G:set var) DA a
+Lemma srd_preservation (E E':onv val) L L' s s' DL (G:set var) DA a e
   (SRD:srd DA s a)
   (RA:rd_agree DA L E)
   (A: AIR2 approx' DA L)
   (LV:live_sound DL s a)
-  (S:F.step (L, E, s) (L',E',s'))
-  : exists DA' DL' a', srd DA' s' a' 
-                   /\ rd_agree DA' L' E' 
+  (S:F.step (L, E, s) e (L',E',s'))
+  : exists DA' DL' a', srd DA' s' a'
+                   /\ rd_agree DA' L' E'
                    /\ AIR2 approx' DL' L'.
 Proof.
   destruct SRD; try inv S.
@@ -619,8 +644,11 @@ Proof.
     rewrite H2 in H7. simpl in *.
     do 3 eexists; repeat split; simpl; eauto.
     pose proof (RA _ _ _ H1 H). simpl in *.
-    eapply rd_agree_update_list; eauto. 
+    eapply rd_agree_update_list; eauto.
     exploit omap_length; eauto. rewrite map_length. congruence.
+
+  + do 2 eexists; repeat split; try eassumption;
+    eauto using agree_on_update_any_same, approx_restrict, rd_agree_update.
 
   + inv LV. do 3 eexists; repeat split; eauto.
     hnf; intros.
@@ -628,7 +656,7 @@ Proof.
     reflexivity.
     eapply RA; eauto.
 
-    econstructor; eauto using agree_on_incl. 
+    econstructor; eauto using agree_on_incl.
     instantiate (1:=Some (getAnn als \ of_list Z)).
     econstructor; eauto.
     split. inv H.
@@ -659,20 +687,20 @@ Inductive srdSim : F.state -> I.state -> Prop :=
   : srdSim (L, E, s) (strip L, EI,s).
 
 Lemma srdSim_sim σ1 σ2
-  : srdSim σ1 σ2 -> sim σ1 σ2.
+  : srdSim σ1 σ2 -> bisim σ1 σ2.
 Proof.
   revert σ1 σ2. cofix; intros.
   destruct H; inv SRD; inv LV; simpl in *; try provide_invariants_2.
-  + case_eq (exp_eval E e); intros.
+  - case_eq (exp_eval E e); intros.
     one_step.
     instantiate (1:=v). erewrite <- exp_eval_live; eauto.
-    eapply srdSim_sim; econstructor; 
+    eapply srdSim_sim; econstructor;
     eauto using approx_restrict, rd_agree_update.
-    eapply agree_on_update_same. reflexivity. 
+    eapply agree_on_update_same. reflexivity.
     eapply agree_on_incl; eauto.
-    eapply simE; try eapply star_refl; eauto; stuck.
+    no_step.
     erewrite <- exp_eval_live in def; eauto. congruence.
-  + case_eq (exp_eval E e); intros.
+  - case_eq (exp_eval E e); intros.
     exploit exp_eval_live_agree; eauto.
     case_eq (val2bool v); intros.
     one_step.
@@ -681,13 +709,13 @@ Proof.
     eapply srdSim_sim; econstructor; eauto using agree_on_incl.
     exploit exp_eval_live_agree; eauto.
     no_step.
-  + no_step. simpl. eapply exp_eval_live; eauto.
-  + decide (length Z0 = length Y).
+  - no_step. simpl. eapply exp_eval_live; eauto.
+  - decide (length Z0 = length Y).
     case_eq (omap (exp_eval E) Y); intros.
-    - exploit omap_exp_eval_live_agree; eauto.
+    + exploit omap_exp_eval_live_agree; eauto.
       pose proof (map_get_1 stripB H1).
       one_step.
-      eapply srdSim_sim. rewrite drop_strip.  
+      eapply srdSim_sim. rewrite drop_strip.
       simpl. simpl counted in *.
       specialize (H3 _ H5); dcr. rewrite H2 in A1,H13.
       econstructor; simpl; eauto using approx_restrict.
@@ -701,36 +729,49 @@ Proof.
       etransitivity; eauto. symmetry. hnf in RA.
       eapply agree_on_incl; eauto.
       exploit omap_length; eauto. rewrite map_length. congruence.
-    - exploit omap_exp_eval_live_agree; eauto.
-      no_step. 
-    - no_step. get_functional; subst; simpl in *; congruence.
+    + exploit omap_exp_eval_live_agree; eauto.
+      no_step.
+    + no_step. get_functional; subst; simpl in *; congruence.
       unfold strip in *.
-      edestruct map_get_4; eauto; dcr; get_functional; subst; simpl in *. 
+      edestruct map_get_4; eauto; dcr; get_functional; subst; simpl in *.
       congruence.
-  + one_step.
+  - extern_step.
+    + exploit omap_exp_eval_live_agree; eauto.
+      eexists; split. econstructor; eauto.
+      eapply srdSim_sim; econstructor; eauto using approx_restrict, rd_agree_update.
+      eapply agree_on_update_same. reflexivity.
+      eapply agree_on_incl; eauto.
+    + symmetry in AG.
+      exploit omap_exp_eval_live_agree; eauto.
+      eexists; split. econstructor; eauto.
+      eapply srdSim_sim; econstructor; eauto using approx_restrict, rd_agree_update.
+      eapply agree_on_update_same. reflexivity.
+      symmetry in AG.
+      eapply agree_on_incl; eauto.
+  - one_step.
     eapply srdSim_sim; econstructor; eauto.
     hnf; intros.
     destruct n; inv H1; inv H2. simpl.
     reflexivity.
-    eapply RA; eauto. 
+    eapply RA; eauto.
 
     econstructor; eauto using agree_on_incl. econstructor; eauto.
-    intros. inv H1. split. 
-    split; cset_tac; isabsurd; eauto. 
+    intros. inv H1. split.
+    split; cset_tac; isabsurd; eauto.
     eexists. split; eauto. cset_tac; intuition.
     decide (a ∈ of_list Z); intuition.
     eapply agree_on_incl; eauto.
 Qed.
 
 Lemma srd_implies_invariance DL s a
-: live_sound DL s a -> params_match nil s -> srd nil s a -> invariant s.
+: live_sound DL s a -> srd nil s a -> invariant s.
 Proof.
-  intros. hnf; intros. eapply srdSim_sim. 
+  intros. hnf; intros. eapply srdSim_sim.
   econstructor; eauto using AIR2; isabsurd; reflexivity.
 Qed.
 
 
-(* 
+(*
 *** Local Variables: ***
 *** coq-load-path: (("." "Lvc")) ***
 *** End: ***
